Weakest-precondition calculus on the minimal language.

proofs/src/dmasm_Mwp.v
@@ -1,11 +1,13 @@
 Require dmasm_Msem.
 
 Import Utf8.
+Import Morphisms.
 Import ssreflect.
 Import ssrbool.
 Import eqtype.
 Import seq.
 Import ZArith.
+Local Open Scope Z_scope.
 
 Import dmasm_utils.
 Import dmasm_type.
@@ -36,7 +38,7 @@ Proof. by move => s s' H; case (msem_inv H). Qed.
 Lemma hoare_skip (Q P: hpred) : Q ⊂ P → hoare Q [::] P.
 Proof. eauto using hoare_conseq, hoare_skip_core. Qed.
 
-Lemma hoare_cons R P Q i c : 
+Lemma hoare_cons R P Q i c :
   hoare P [:: i] R →  hoare R c Q →  hoare P (i :: c) Q.
 Proof.
   by
@@ -56,6 +58,326 @@ Proof.
   case: (msem_I_inv Hi) => v [ Hv Hs' ].
   firstorder.
 Qed.
+
+(* WP *)
+(* A formula is a predicate over an environment that maps logical variables to value. *)
+(* This predicate should be extensional *)
+
+Definition env : Type := Mv.t ssem_t.
+Definition env_ext (m m': env) : Prop :=
+  ∀ x, (m.[x] = m'.[x])%mv.
+
+Definition env_ext_refl m : env_ext m m := λ x, Logic.eq_refl.
+Definition env_ext_sym m m' (H: env_ext m m') : env_ext m' m :=
+  λ x, Logic.eq_sym (H x).
+Definition env_ext_trans m' m m'' (H: env_ext m m') (H': env_ext m' m'') :
+  env_ext m m'' :=
+  λ x, Logic.eq_trans (H x) (H' x).
+
+Lemma env_ext_empty m m' :
+  (∀ x, m x = m' x) →
+  env_ext (Mv.empty m) (Mv.empty m').
+Proof. by move=> E x; rewrite ! Mv.get0. Qed.
+
+Lemma env_ext_set m m' x v :
+  env_ext m m' →
+  (env_ext (m.[x <- v]) (m'.[x <- v]))%mv.
+Proof.
+  move=> E y.
+  case: (x =P y) => [ <- | H ].
+  rewrite ! Mv.setP_eq //.
+  rewrite ! Mv.setP_neq //;
+  case: eqP => //.
+Qed.
+
+Definition formula : Type :=
+  sigT (Proper (env_ext ==> iff)).
+
+Lemma formula_m (f: env → Prop) :
+  (∀ s s', env_ext s s' → f s → f s') →
+  Proper (env_ext ==> iff) f.
+Proof.
+  move=> E s s' H.
+  split; eauto using env_ext_sym.
+Qed.
+
+Instance constant_formula_m (P: Prop) : Proper (env_ext ==> iff) (λ _, P) :=
+  formula_m _ (λ _ _ _ (p: P), p).
+
+Example ftrue: formula := existT _ (λ _, True) _.
+Example ffalse: formula := existT _ (λ _, False) _.
+
+Definition formula_of_hpred (P: hpred) : formula.
+Proof.
+  refine (existT _ (λ s: env, P (Fv.empty (λ x, s.[x])%mv)) _).
+  apply formula_m.
+  move=> s s' E H.
+  refine (eq_ind _ P H _ _).
+  apply Fv.map_ext. auto.
+Defined.
+
+Notation "⟨ P ⟩" := (formula_of_hpred P) : msem_scope.
+
+Definition formula_denote (f: formula) : hpred :=
+  λ s, projT1 f (Mv.empty (λ x, s.[x])%vmap).
+
+Notation "⟦ f ⟧" := (formula_denote f) : msem_scope.
+
+Lemma formula_of_hpred_denote P :
+  ∀ s, ⟦ ⟨P⟩ ⟧ s ↔ P s.
+Proof.
+  unfold formula_of_hpred, formula_denote. simpl.
+  by
+  move=> s; split; move=> H; refine (eq_ind _ P H _ _); apply Fv.map_ext; move=> x;
+  rewrite Fv.get0 Mv.get0.
+Qed.
+
+Inductive texpr : stype → Type :=
+| Tvar v : texpr (vtype v)
+| Tconst `(Z) : texpr sint
+| Tbool `(bool) : texpr sbool
+| Tadd (_ _: texpr sint) : texpr sint
+| Tand (_ _: texpr sbool) : texpr sbool
+.
+
+Section SEM_TEXPR.
+  Context (m: Mv.t ssem_t).
+  Fixpoint sem_texpr ty (e: texpr ty) : ssem_t ty :=
+    match e with
+    | Tvar x => m.[x]
+    | Tconst z => z
+    | Tbool b => b
+    | Tadd p q => sem_texpr sint p + sem_texpr sint q
+    | Tand p q => sem_texpr sbool p && sem_texpr sbool q
+    end%mv.
+End SEM_TEXPR.
+
+Lemma sem_texpr_m (s s': env) :
+  env_ext s s' →
+  ∀ ty e, sem_texpr s ty e = sem_texpr s' ty e.
+Proof.
+  move=> E ty e.
+  elim: e => //; simpl; congruence.
+Qed.
+
+Definition stype_eq_dec (ty ty': stype) : { ty = ty' } + { True } :=
+  match ty, ty' with
+  | sint, sint => left Logic.eq_refl
+  | sbool, sbool => left Logic.eq_refl
+  | _, _ => right I
+  end.
+
+Fixpoint type_check_mexpr (e: mexpr) (ty: stype) : option (texpr ty) :=
+  match e with
+  | Mvar x =>
+    match stype_eq_dec (vtype x) ty with
+    | left EQ => Some (eq_rect _ _ (Tvar x) _ EQ)
+    | right _ => None
+    end
+  | Mconst z => match ty with sint => Some (Tconst z) | _ => None end
+  | Mbool b => match ty with sbool => Some (Tbool b) | _ => None end
+  | Madd p q =>
+    match type_check_mexpr p sint with
+    | Some tp =>
+    match type_check_mexpr q sint with
+    | Some tq => match ty with sint => Some (Tadd tp tq) | _ => None end
+    | None => None end
+    | None => None end
+  | Mand p q =>
+    match type_check_mexpr p sbool with
+    | Some tp =>
+    match type_check_mexpr q sbool with
+    | Some tq => match ty with sbool => Some (Tand tp tq) | _ => None end
+    | None => None end
+    | None => None end
+  end.
+
+Definition Some_inj {A} (a a': A) (H: Some a = Some a') : a = a' :=
+  let 'Logic.eq_refl := H in Logic.eq_refl.
+
+Definition ok_inj {E A} (a a': A) (H: Ok E a = ok a') : a = a' :=
+  let 'Logic.eq_refl := H in Logic.eq_refl.
+
+Lemma of_sval_to_sval ty x :
+  of_sval ty (to_sval x) = ok x.
+Proof. by move: x; case ty. Qed.
+
+Lemma sto_int_inv x i :
+  sto_int x = ok i →
+  x = i.
+Proof. case: x => // i' H; apply ok_inj in H. congruence. Qed.
+
+Lemma sto_bool_inv x b :
+  sto_bool x = ok b →
+  x = b.
+Proof. case: x => // i' H; apply ok_inj in H. congruence. Qed.
+
+Lemma type_check_mexprP {e ty te} :
+  type_check_mexpr e ty = Some te →
+  ∀ s v,
+  msem_mexpr s e = ok v →
+  ∀ s',
+  (∀ x, s.[x]%vmap = s'.[x]%mv) →
+  of_sval _ v = ok (sem_texpr s' ty te).
+Proof.
+  elim: e ty te.
+  - move=> v ty te. simpl. case: stype_eq_dec => //.
+    move=> EQ H; apply Some_inj in H; subst.
+    move=> s v' H; apply ok_inj in H; subst v'.
+    move=> s' E. simpl. unfold sget_var. rewrite E.
+    apply of_sval_to_sval.
+  - move=> z [] // te H; apply Some_inj in H; subst.
+    move=> s v H; apply ok_inj in H; subst v.
+    reflexivity.
+  - move=> b [] // te H; apply Some_inj in H; subst.
+    move=> s v H; apply ok_inj in H; subst v.
+    reflexivity.
+  - move=> p IHp q IHq ty te.
+    simpl.
+    move: (IHp sint). clear IHp.
+    case: (type_check_mexpr p _) => // tp IHp.
+    specialize (IHp _ Logic.eq_refl).
+    move: (IHq sint). clear IHq.
+    case: (type_check_mexpr q _) => // tq IHq.
+    specialize (IHq _ Logic.eq_refl).
+    move: te. case: ty => // te H; apply Some_inj in H; subst.
+    move=> s v.
+    move=> H; case: (bindW H) => vp Ep. clear H.
+    move=> H; case: (bindW H) => vq Eq. clear H.
+    move=> H; case: (bindW H) => ip Tp. clear H.
+    move=> H; case: (bindW H) => iq Tq. clear H.
+    move=> H; apply ok_inj in H; subst.
+    move=> s' E. simpl.
+    specialize (IHp _ _ Ep _ E).
+    specialize (IHq _ _ Eq _ E).
+    apply sto_int_inv in IHp.
+    apply sto_int_inv in IHq.
+    apply sto_int_inv in Tp.
+    apply sto_int_inv in Tq. congruence.
+  - move=> p IHp q IHq ty te.
+    simpl.
+    move: (IHp sbool). clear IHp.
+    case: (type_check_mexpr p _) => // tp IHp.
+    specialize (IHp _ Logic.eq_refl).
+    move: (IHq sbool). clear IHq.
+    case: (type_check_mexpr q _) => // tq IHq.
+    specialize (IHq _ Logic.eq_refl).
+    move: te. case: ty => // te H; apply Some_inj in H; subst.
+    move=> s v.
+    move=> H; case: (bindW H) => vp Ep. clear H.
+    move=> H; case: (bindW H) => vq Eq. clear H.
+    move=> H; case: (bindW H) => bp Tp. clear H.
+    move=> H; case: (bindW H) => bq Tq. clear H.
+    move=> H; apply ok_inj in H; subst.
+    move=> s' E. simpl.
+    specialize (IHp _ _ Ep _ E).
+    specialize (IHq _ _ Eq _ E).
+    apply sto_bool_inv in IHp.
+    apply sto_bool_inv in IHq.
+    apply sto_bool_inv in Tp.
+    apply sto_bool_inv in Tq. congruence.
+Qed.
+
+Definition wp_assgn (x: var) (e: mexpr) (f: formula) : formula.
+  refine
+  match type_check_mexpr e (vtype x) with
+  | Some te =>
+    existT _ (
+    λ s,
+    ∀ v, sem_texpr s (vtype x) te = v → projT1 f (s.[x <- v])%mv) _
+  | None => ffalse
+  end.
+Proof.
+  abstract (
+  apply formula_m;
+  move=> s s' E X v V;
+  rewrite (projT2 f); [| apply env_ext_set, env_ext_sym, E ];
+  apply X; etransitivity; [ apply sem_texpr_m, E | exact V ]).
+Defined.
+
+Lemma wp_assgn_sound x e f :
+  hoare ⟦wp_assgn x e f⟧ [:: MCassgn x e] ⟦f⟧.
+Proof.
+  move=> s s1 /msem_inv [s' [H' /msem_inv]] ->.
+  case: (msem_I_inv H') => v [Hv H]. clear H'.
+  case: (bindW H) => [u Hu Hs']. clear H.
+  apply ok_inj in Hs'. subst s'.
+  unfold wp_assgn.
+  case (type_check_mexpr _ _) eqn: EQ. 2: firstorder.
+  move: (type_check_mexprP EQ _ _ Hv) => R.
+  unfold formula_denote. simpl.
+  move=> X.
+  rewrite (projT2 f). apply X. clear X.
+  Focus 2.
+  move=> y. rewrite Mv.get0.
+  case: (x =P y).
+  move=> <-. rewrite ! (Fv.setP_eq, Mv.setP_eq). reflexivity.
+  move=> NE. rewrite ! (Fv.setP_neq, Mv.setP_neq) //; case: eqP => //.
+  apply: ok_inj. etransitivity. 2: apply Hu.
+  symmetry. apply R.
+  auto.
+Qed.
+
+Definition wp_minstr (i: minstr) (f: formula) : formula :=
+  match i with
+  | MCassgn x e => wp_assgn x e f
+  end.
+
+Lemma wp_minstr_sound i f :
+  hoare ⟦wp_minstr i f⟧ [:: i] ⟦f⟧.
+Proof.
+  case i => x e.
+  apply: wp_assgn_sound.
+Qed.
+
+Definition wp (c: mcmd) (f: formula) : formula :=
+  foldr wp_minstr f c.
+
+Lemma wp_sound c f :
+  hoare ⟦wp c f⟧ c ⟦f⟧.
+Proof.
+  elim: c f.
+  - auto using hoare_skip_core.
+  - simpl; eauto using wp_minstr_sound, hoare_cons.
+Qed.
+
+Print Assumptions wp_sound.
+
+Lemma hoare_by_wp (P: hpred) c Q :
+  P ⊂ ⟦wp c ⟨Q⟩⟧ →
+  hoare P c Q.
+Proof.
+  move=> E.
+  eapply hoare_conseq. exact E. 2: apply wp_sound.
+  apply formula_of_hpred_denote.
+Qed.
+
+Section Example.
+  Let x : var := Var sint "x".
+  Let y : var := Var sint "y".
+
+  Let p : mcmd :=
+    MCassgn x (Mconst 1)
+ :: MCassgn x (Madd (Mvar x) (Mconst 1))
+ :: MCassgn y (Madd (Mvar x) (Mvar x))
+ :: MCassgn x (Madd (Mvar y) (Mvar y))
+ :: MCassgn y (Madd (Mvar x) (Mvar x))
+ :: MCassgn x (Madd (Mvar y) (Mvar y))
+ :: MCassgn y (Madd (Mvar x) (Mvar x))
+ :: MCassgn x (Madd (Mvar y) (Mvar y))
+ :: nil.
+
+  Goal hoare (λ _, True) p (λ e, Z.even e.[x]%vmap).
+  Proof.
+    apply hoare_by_wp. move=> q _.
+    simpl. setoid_rewrite Mv.setP_eq.
+    intuition subst.
+    reflexivity.
+  Abort.
+
+End Example.
+
+(*
 
 (* WP *)
 (* A “formula” is a list of variables and a predicate over the values of these variables *)
@@ -130,7 +452,7 @@ Section Example0.
 End Example0.
 
 (* λ v1 … vn w1 … wn,
-∀ x, x = ⟦e⟧ v1 … vn → ⟦f⟧^x x w1 … wn 
+∀ x, x = ⟦e⟧ v1 … vn → ⟦f⟧^x x w1 … wn
  *)
 Definition wp_assgn (x: var) (e: mexpr) (f: formula) : formula :=
   if true then
@@ -165,3 +487,5 @@ Proof.
   - auto using hoare_skip_core.
   - simpl; eauto using wp_minstr_sound, hoare_cons.
 Qed.
+
+*)
